theories/SemanticsSpec.v
@@ -327,7 +327,6 @@ Inductive eval (locals : @Ident.Map.t value) : heap -> t -> heap -> value -> Pro
   eval locals h (Mblock (tag, es)) h' (Block (tag, vals))
 | eval_field h h' idx b vals tag :
   eval locals h b h' (Block (tag, vals)) ->
-  Datatypes.length vals < Z.to_nat Int63.wB ->
   Datatypes.length vals <= int_to_nat max_length ->
   int_to_nat idx < List.length vals ->
   eval locals h (Mfield (idx, b)) h' (nth (int_to_nat idx) vals (fail ""))
@@ -366,7 +365,8 @@ Inductive eval (locals : @Ident.Map.t value) : heap -> t -> heap -> value -> Pro
 | eval_num_int n h : eval locals h (Mnum (numconst_Int n)) h (value_Int (Int, Int63.to_Z n))
 | eval_num_bigint n h : eval locals h (Mnum (numconst_Bigint n)) h  (value_Int (Bigint, n))
 | eval_num_float f h : eval locals h (Mnum (numconst_Float64 f)) h  (Float f)
-| eval_string (s:string) h h' h'' ptr : 
+| eval_string s h h' h'' ptr : 
+  String.length s < int_to_nat max_length ->
   let str := init (String.length s)
     (fun i => value_Int (Int, Z.of_nat (Byte.to_nat (option_def (Ascii.byte_of_ascii Ascii.Space) (get i s))))) in
   fresh h ptr h' -> 
@@ -446,13 +446,18 @@ Inductive eval (locals : @Ident.Map.t value) : heap -> t -> heap -> value -> Pro
                   h' (Float (as_float v))                                              
 | eval_vecnew_array h h1 h2 h3 h4 len len' def def' ptr : 
       eval locals h len h1 (value_Int (Int, len')) -> 
+      (0 <= len')%Z ->
+      Z.to_nat len' <= int_to_nat max_length ->
       eval locals h1 def h2 def' ->
       fresh h2 ptr h3 -> 
       update h3 ptr (init (Z.to_nat len') (fun _ => def')) h4 ->
       eval locals h (Mvecnew (Array, len, def)) h4 (Vec (Array, ptr))
 | eval_vecnew_bytevec h h1 h2 h3 h4 len len' def k ptr : 
       eval locals h len h1 (value_Int (Int, len')) -> 
+      (0 <= len')%Z ->
+      Z.to_nat len' <= int_to_nat max_length ->
       eval locals h1 def h2 (value_Int (Int, k)) ->
+      is_true (Z.leb 0%Z k && Z.ltb k 256) ->
       fresh h2 ptr h3 -> 
       update h3 ptr (init (Z.to_nat len') (fun _ => (value_Int (Int, k)))) h4 ->
       eval locals h (Mvecnew (Bytevec, len, def)) 
@@ -476,26 +481,36 @@ Inductive eval (locals : @Ident.Map.t value) : heap -> t -> heap -> value -> Pro
        | _ => fail "wrong vector type"
        end)
   | eval_vecset h h1 h2 h3 h4 vec ty ty' ptr idx i e v arr :  
-  eval locals h vec h1 (Vec (ty', ptr)) -> 
-  eval locals h1 idx h2 (value_Int (Int, i)) ->
-  eval locals h2 e h3 v ->
-  deref h ptr arr -> 
-  update h3 ptr (set arr (Z.to_nat i) v) h4 ->
-  eval locals h (Mvecset (ty, vec, idx, e)) 
-              h4 (if vector_type_eqb ty ty' then 
-        let i := Int63.of_Z i in 
-        if Int63.leb (int_of_nat 0) i && Int63.leb i (int_of_nat (List.length arr)) then 
-          match ty, v with 
-          | Array, _ => value_Int (Int, 0%Z)
-          | Bytevec, value_Int (Int, val) => 
-            if (Z.leb 0 val) && (Z.ltb val 256)
-            then 
-              value_Int (Int, 0%Z)
-            else fail "not a byte"
-          | Bytevec, _ => fail "not a byte"
-          end 
-        else fail "index out of bounds: %d"
-    else fail "wrong vector type")  
+    eval locals h vec h1 (Vec (ty', ptr)) -> 
+    eval locals h1 idx h2 (value_Int (Int, i)) ->
+    eval locals h2 e h3 v ->
+    deref h ptr arr -> 
+    update h3 ptr (set arr (Z.to_nat i) v) h4 ->
+    eval locals h (Mvecset (ty, vec, idx, e)) 
+        (if vector_type_eqb ty ty' then 
+           if Z.leb 0 i && Z.ltb i (Z.of_nat (List.length arr)) then 
+             match ty, v with 
+              | Array, _ => h4
+              | Bytevec, value_Int (Int, val) => 
+                if (Z.leb 0 val) && (Z.ltb val 256)
+                then h4
+                else h3
+              | Bytevec, _ => h3
+              end 
+            else h3
+          else h3)
+        (if vector_type_eqb ty ty' then 
+           if Z.leb 0 i && Z.ltb i (Z.of_nat (List.length arr)) then 
+             match ty, v with 
+              | Array, _ => value_Int (Int, 0%Z)
+              | Bytevec, value_Int (Int, val) => 
+                  if (Z.leb 0 val) && (Z.ltb val 256)
+                  then value_Int (Int, 0%Z)
+                  else fail "not a byte"
+              | Bytevec, _ => fail "not a byte"
+            end 
+           else fail "index out of bounds: %d"
+         else fail "wrong vector type")  
 | eval_veclen h h' vec ty' ptr ty arr : 
   eval locals h vec h' (Vec (ty', ptr)) -> 
   deref h ptr arr -> 
@@ -597,7 +612,6 @@ forall P : Ident.Map.t -> heap -> t -> heap -> value -> Prop,
           (tag : Malfunction.int),
         eval locals h b h' (Block (tag, vals)) ->
         P locals h b h' (Block (tag, vals)) ->
-        Datatypes.length vals < Z.to_nat Int63.wB ->
         Datatypes.length vals <= int_to_nat max_length ->
         int_to_nat idx < Datatypes.length vals ->
         P locals h (Mfield (idx, b)) h' (nth (int_to_nat idx) vals (fail ""))) ->
@@ -649,6 +663,7 @@ forall P : Ident.Map.t -> heap -> t -> heap -> value -> Prop,
         P locals h (Mnum (numconst_Float64 f21)) h (Float f21)) ->
        (forall (locals : Ident.Map.t) (s : string) 
           (h h' h'' : heapGen value) (ptr : pointer),
+        String.length s < int_to_nat max_length ->
         let str :=
           init (String.length s)
             (fun i : nat =>
@@ -768,6 +783,8 @@ forall P : Ident.Map.t -> heap -> t -> heap -> value -> Prop,
           (h3 h4 : heapGen value) (len : t) (len' : Z) 
           (def : t) (def' : value) (ptr : pointer),
         eval locals h len h1 (value_Int (Int, len')) ->
+        (0 <= len')%Z -> 
+        Z.to_nat len' <= int_to_nat max_length ->
         P locals h len h1 (value_Int (Int, len')) ->
         eval locals h1 def h2 def' ->
         P locals h1 def h2 def' ->
@@ -778,8 +795,11 @@ forall P : Ident.Map.t -> heap -> t -> heap -> value -> Prop,
           (h3 h4 : heapGen value) (len : t) (len' : Z) 
           (def : t) (k : Z) (ptr : pointer),
         eval locals h len h1 (value_Int (Int, len')) ->
+        (0 <= len')%Z -> 
+        Z.to_nat len' <= int_to_nat max_length ->
         P locals h len h1 (value_Int (Int, len')) ->
         eval locals h1 def h2 (value_Int (Int, k)) ->
+        is_true (Z.leb 0%Z k && Z.ltb k 256) ->
         P locals h1 def h2 (value_Int (Int, k)) ->
         fresh h2 ptr h3 ->
         update h3 ptr
@@ -821,27 +841,31 @@ forall P : Ident.Map.t -> heap -> t -> heap -> value -> Prop,
         P locals h2 e h3 v ->
         deref h ptr arr ->
         update h3 ptr (set arr (Z.to_nat i) v) h4 ->
-        P locals h (Mvecset (ty, vec, idx, e)) h4
-          (if vector_type_eqb ty ty'
-           then
-            let i0 := Int63.of_Z i in
-            if
-             ((int_of_nat 0 ≤? i0)%uint63 &&
-              (i0 ≤? int_of_nat (Datatypes.length arr))%uint63)%bool
-            then
-             match ty with
-             | Array => value_Int (Int, 0%Z)
-             | Bytevec =>
-                 match v with
-                 | value_Int (Int, val) =>
-                     if ((0 <=? val)%Z && (val <? 256)%Z)%bool
-                     then value_Int (Int, 0%Z)
-                     else fail "not a byte"
-                 | _ => fail "not a byte"
-                 end
-             end
-            else fail "index out of bounds: %d"
-           else fail "wrong vector type")) ->
+        P locals h (Mvecset (ty, vec, idx, e)) 
+        (if vector_type_eqb ty ty' then 
+           if Z.leb 0 i && Z.ltb i (Z.of_nat (List.length arr)) then 
+             match ty, v with 
+              | Array, _ => h4
+              | Bytevec, value_Int (Int, val) => 
+                if (Z.leb 0 val) && (Z.ltb val 256)
+                then h4
+                else h3
+              | Bytevec, _ => h3
+              end 
+            else h3
+          else h3)
+        (if vector_type_eqb ty ty' then 
+           if Z.leb 0 i && Z.ltb i (Z.of_nat (List.length arr)) then 
+             match ty, v with 
+              | Array, _ => value_Int (Int, 0%Z)
+              | Bytevec, value_Int (Int, val) => 
+                  if (Z.leb 0 val) && (Z.ltb val 256)
+                  then value_Int (Int, 0%Z)
+                  else fail "not a byte"
+              | Bytevec, _ => fail "not a byte"
+            end 
+           else fail "index out of bounds: %d"
+         else fail "wrong vector type")) ->
        (forall (locals : Ident.Map.t) (h h' : heap) 
           (vec : t) (ty' : vector_type) (ptr : pointer) 
           (ty : vector_type) (arr : list value),
