theories/utils_array.v
@@ -1,0 +1,157 @@
+Require Import ssreflect.
+
+Require Import ZArith Array.PArray List Floats Lia.
+Import ListNotations.
+
+Require Import Malfunction.Malfunction Malfunction.SemanticsSpec.
+From Coq Require Import Uint63.
+
+Fixpoint Array_of_List' {A} count (l : list A) (a : array A) :=
+  match l with
+  | [] => a
+  | x :: l => Array_of_List' (S count) l (PArray.set a (int_of_nat count) x)
+  end.
+
+Definition Array_of_list {A} (def : A) (l : list A) :=
+  Array_of_List' 0 l (PArray.make (int_of_nat (List.length l)) def).
+
+Definition Array_init {A} (size : int) f :=
+  let g := fun x => (f (int_of_nat x)) in
+  @Array_of_list A (g 0) (map g (seq 0 (Z.to_nat (Int63.to_Z size)))).
+
+
+Lemma Array_of_list'_get {A} s l (a : array A) i :
+  i < s + List.length l ->
+  (s + List.length l < Z.to_nat Int63.wB) ->
+  s + List.length l <= int_to_nat (PArray.length a) ->
+  PArray.get (Array_of_List' s l a) (int_of_nat i) =
+    if (i <? s)%nat then
+      a.[int_of_nat i]
+    else
+      nth (i - s) l (a.[int_of_nat i]).
+Proof.
+  intros Hl Hs Ha.
+  induction l as [ | ? ? IHl] in s, i, a, Hl, Hs, Ha |- *.
+  - destruct (Nat.ltb_spec i s).
+    + cbn. reflexivity.
+    + cbn. destruct (i - s); reflexivity.
+  - rewrite IHl. 
+    + cbn in Hl. lia.
+    + cbn [Datatypes.length] in Hs. lia.
+    + rewrite PArray.length_set. cbn [Datatypes.length] in Ha. lia.
+    + fold (int_of_nat s). destruct (Nat.ltb_spec i s) as [H | H].
+      * destruct (Nat.ltb_spec i (S s)) as [H0 | H0]; try lia.
+        rewrite get_set_other.
+        -- intros E. eapply (f_equal int_to_nat) in E.
+           rewrite !int_to_of_nat in E.
+           all:assert (H1 : s < Z.to_nat Int63.wB) by lia.
+           all:eapply inj_lt in H1.
+           all:rewrite Z2Nat.id in H1. all:lia. 
+        -- reflexivity.
+      * destruct (Nat.ltb_spec i (S s)); try lia.
+        -- assert (i = s) by lia. subst.
+           rewrite get_set_same.
+           ++ eapply Int63.ltb_spec.
+              1:eapply Z2Nat.inj_lt.
+              1:eapply Int63.to_Z_bounded.
+              1:eapply Int63.to_Z_bounded. 
+              fold (int_to_nat (int_of_nat s)).
+              rewrite int_to_of_nat. 1:lia.
+              unfold int_to_nat in Ha. lia.
+           ++ cbn. destruct s. 1:reflexivity.
+              rewrite Nat.sub_diag. reflexivity.
+        -- cbn. destruct (i - s) as [ | n] eqn:E.
+           ++ lia.
+           ++ assert (H1 : i - S s = n) by lia. rewrite H1.
+              eapply nth_indep.
+              cbn in Hl. lia.
+Qed.
+
+Lemma Array_of_list_get {A} (a : A) l i :
+  (i < Z.to_nat Int63.wB) ->
+  (List.length l < Z.to_nat Int63.wB) ->
+  List.length l <= int_to_nat max_length ->
+  i < List.length l ->
+  (Array_of_list a l).[int_of_nat i] = nth i l a.
+
+Proof.
+  unfold Array_of_list. intros Hs Hl1 Hl Hi.
+  rewrite Array_of_list'_get.
+  + assumption.
+  + lia. 
+  + rewrite PArray.length_make.
+    fold (int_of_nat (Datatypes.length l)).
+    destruct (Int63.lebP (int_of_nat (Datatypes.length l)) max_length) as [ | n ].
+    * rewrite int_to_of_nat.
+      1:eapply Z2Nat.inj_lt. all: lia. 
+    * destruct n.
+      epose proof (int_to_of_nat (Datatypes.length l) _) as H.
+      eapply Z2Nat.inj_le.
+      1:eapply Int63.to_Z_bounded.
+      1:eapply Int63.to_Z_bounded.
+      unfold int_to_nat in H. rewrite H.
+      unfold int_to_nat in Hl. exact Hl.
+      Unshelve. all:lia.
+  + destruct (Nat.ltb_spec i 0); try lia.
+    rewrite Nat.sub_0_r.
+    eapply nth_indep. lia.
+Qed.
+
+
+Lemma Array_of_list_get_again {A : Set} i s (l : list A) a :
+  i >= s + List.length l ->
+  s + List.length l < Z.to_nat Int63.wB ->
+  i < Z.to_nat Int63.wB ->
+  (Array_of_List' s l a).[int_of_nat i]  = PArray.get a (int_of_nat i).
+Proof.
+  induction l as [ | ? l IHl ] in s, i, a |- *; intros Hi Hs Ha.
+  - cbn. reflexivity.
+  - cbn. rewrite IHl. 
+    + cbn in Hi. lia.
+    + cbn [List.length] in Hs. lia. 
+    + cbn [List.length] in Hs. lia.
+    + rewrite get_set_other. 2:reflexivity.
+      fold (int_of_nat s).
+      intros H. eapply (f_equal int_to_nat) in H.
+      rewrite !int_to_of_nat in H.
+      * eapply inj_lt in Hs.
+        rewrite Z2Nat.id in Hs. 1:cbn; lia.
+        rewrite <- Hs.
+        eapply inj_lt. cbn. lia.
+      * eapply inj_lt in Ha.
+        rewrite Z2Nat.id in Ha. 1:cbn; lia.
+        lia.
+      * subst. cbn in Hi. lia.
+Qed.
+
+
+Lemma Array_of_list_S A default n a (l:list A) : 
+  n < Datatypes.length l ->
+  S (Datatypes.length l) <= int_to_nat max_length ->
+  (Array_of_list default (a :: l)).[int_of_nat (S n)] = 
+  (Array_of_list default l).[int_of_nat n].
+Proof.
+  intros. 
+  repeat rewrite Array_of_list_get; cbn in *; try lia; eauto.
+Qed.
+
+Lemma Array_of_list'_length A k (l:list A) a :
+  PArray.length (Array_of_List' k l a) =
+  PArray.length a.
+Proof. 
+  revert k a. induction l; [reflexivity|].
+  intros; cbn. rewrite IHl. now rewrite PArray.length_set.
+Qed.
+
+Lemma Array_of_list_length A default (l:list A) :
+  Datatypes.length l < int_to_nat max_length -> 
+  int_to_nat (PArray.length (Array_of_list default l)) =
+  List.length l.
+Proof.
+  unfold Array_of_list. rewrite Array_of_list'_length.
+  rewrite PArray.length_make. intro H. 
+  assert (Hl: (int_of_nat (Datatypes.length l) ≤? max_length)%uint63 = true).
+  { apply leb_spec. rewrite Int63.of_Z_spec. rewrite Z.mod_small; [cbn in *; lia |].
+    cbn in *; lia. }
+  rewrite Hl. apply int_to_of_nat. cbn in *; lia. 
+Qed.
